proof/auditor_proof/base.v
@@ -5,6 +5,9 @@ From New.proof Require Import bytes sync.
 From New.proof.github_com.sanjit_bhat.pav Require Import
   advrpc cryptoffi hashchain ktcore merkle safemarshal server.
 
+(* TODO: upstream. *)
+#[global] Opaque rwmutex.actualMaxReaders.
+
 Module auditor.
 Section proof.
 Context `{hG: heapGS Σ, !ffi_semantics _ _, !globalsGS Σ} {go_ctx : GoContext}.
